src/Dafny/examples/fs/byte_fs.dfy
@@ -107,7 +107,9 @@ module ByteFs {
 
   lemma write_data_app(data: seq<byte>, off: nat, bs1: seq<byte>, bs2: seq<byte>)
     requires off <= |data|
-    ensures write_data(data, off, bs1 + bs2) == write_data(write_data(data, off, bs1), off + |bs1|, bs2)
+    ensures write_data(data, off, bs1 + bs2) ==
+        write_data(write_data(data, off, bs1),
+          off + |bs1|, bs2)
   {}
 
   class ByteFilesys
